I will proceed to prove M is sound and complete wrt dual models.

Modal/modal/logics/logic_E.lean
@@ -8,7 +8,7 @@ open ModalAxioms ModalRules CPLSeq ModalFormula
 variable {α : Type} [ModalSyntax α]
 
 inductive EProof : ModalFormula α → Prop where
-  | classical {p : ModalFormula α} (h_cpl : CPLProof p) : EProof p
+  | cpl {p : ModalFormula α} (h_cpl : CPLProof p) : EProof p
   | rl_re {p q : ModalFormula α} (h_prem : EProof (rl_re p q).premise) :
                                            EProof (rl_re p q).conclusion
-  | ax_def_dia {p : ModalFormula α} : EProof (ax_def_dia p)
+  | ax_dia {p : ModalFormula α} : EProof (ax_dia p)
