Modal/modal/axioms_rules.lean
@@ -9,7 +9,7 @@ namespace ModalRules
 
 variable {φ : Type} [ModalSyntax φ]
 
-def rl_nec (p : φ) : InferenceRule1 φ := ⟨p, □p⟩
+def rl_nec (p : φ) : InferenceRule1 φ  := ⟨p, □p⟩
 def rl_re (p q : φ) : InferenceRule1 φ := ⟨p ↔ q, □p ↔ □q⟩
 
 end ModalRules
@@ -20,18 +20,12 @@ namespace ModalAxioms
 variable {φ : Type} [ModalSyntax φ]
 
 def ax_dia (p : φ) : φ := ◇p ↔ ¬□¬p
-def ax_T (p : φ) : φ := □p → p
-def ax_B (p : φ) : φ := p → □(◇p)
-def ax_4 (p : φ) : φ := □p → □(□p)
-def ax_5 (p : φ) : φ := ◇p → □(◇p)
-def ax_M (p q : φ) : φ := □(p∧q) ↔ □p
-
-def ax_K (p q : φ) : φ := □(p → q) → (□p → □q)
-def ax_K_b (p q : φ) : φ := ax_K p q
-def ax_K_d (p q : φ) : φ := ◇(p → q) → (◇p → ◇q)
-def ax_N : φ := □⊤
-def ax_N_b : φ := ax_N
-def ax_N_d : φ := ◇⊤
-def ax_KN2 (p q : φ) : φ := ((ax_K_b p q) ∧ ax_N_b) ∨ ((ax_K_d p q) ∧ ax_N_d)
+def ax_t (p : φ) : φ   := □p → p
+def ax_b (p : φ) : φ   := p → □(◇p)
+def ax_4 (p : φ) : φ   := □p → □(□p)
+def ax_5 (p : φ) : φ   := ◇p → □(◇p)
+def ax_m (p q : φ) : φ := □(p∧q) ↔ □p
+def ax_k (p q : φ) : φ := □(p → q) → (□p → □q)
+def ax_n : φ           := □⊤
 
 end ModalAxioms
