Modal/modal/logics/logic_M.lean
@@ -1,0 +1,15 @@
+import Modal.cpl.proof
+import Modal.modal.formula
+import Modal.modal.axioms_rules
+
+
+open ModalAxioms ModalRules CPLSeq ModalFormula
+
+variable {α : Type} [ModalSyntax α]
+
+inductive MProof : ModalFormula α → Prop where
+  | cpl {p : ModalFormula α} (h_cpl : CPLProof p) : MProof p
+  | rl_re {p q : ModalFormula α} (h_prem : MProof (rl_re p q).premise) :
+                                           MProof (rl_re p q).conclusion
+  | ax_dia {p : ModalFormula α} : MProof (ax_dia p)
+  | ax_m {p q : ModalFormula α} : MProof (ax_m p q)
