Modal/modal/sound-complete/logicE_nbhd.lean
@@ -1,0 +1,14 @@
+import Modal.modal.formula
+import Modal.modal.models.nbhd
+import Modal.modal.logics.logic_E
+
+
+open ModalFormula
+
+
+variable {α : Type}
+
+-- well-known result
+theorem logicE_nbhd_sc :
+    ∀ (φ : ModalFormula α), Neighborhood.valid φ ↔ EProof φ := by
+    sorry
