Modal/modal/sound-complete/logicM_dual.lean
@@ -1,0 +1,24 @@
+import Modal.modal.formula
+import Modal.modal.models.dual
+import Modal.modal.logics.logic_M
+
+
+open ModalFormula Dual
+
+
+variable {α : Type}
+
+theorem logicM_dual_sound :
+    ∀ (φ : ModalFormula α), MProof φ → valid φ := by
+    sorry
+
+theorem logicM_dual_complete :
+    ∀ (φ : ModalFormula α), valid φ → MProof φ := by
+    sorry
+
+theorem logicM_dual_sc :
+    ∀ (φ : ModalFormula α), valid φ ↔ MProof φ := by
+    intro φ
+    constructor
+    · exact logicM_dual_complete φ
+    · exact logicM_dual_sound φ
