Modal/modal/sound-complete/logicM_upnbhd.lean
@@ -1,0 +1,14 @@
+import Modal.modal.formula
+import Modal.modal.models.nbhd
+import Modal.modal.logics.logic_M
+
+
+open ModalFormula Neighborhood
+
+
+variable {α : Type}
+
+-- well-known result
+theorem logicM_upnbhd_sc :
+    ∀ (φ : ModalFormula α), valid_in_class IsUpwardClosed φ ↔ MProof φ := by
+    sorry
